Fix bench failure due to the new Bag theory.

examples/programs/vstte12_bfs/vstte12_bfs_WP_BFS_WP_parameter_bfs_1.v
@@ -3,18 +3,19 @@
 Require Import ZArith.
 Require Import Rbase.
 Require int.Int.
+
+(* Why3 assumption *)
 Definition unit  := unit.
 
 Parameter qtmark : Type.
 
 Parameter at1: forall (a:Type), a -> qtmark -> a.
-
 Implicit Arguments at1.
 
 Parameter old: forall (a:Type), a -> a.
-
 Implicit Arguments old.
 
+(* Why3 assumption *)
 Definition implb(x:bool) (y:bool): bool := match (x,
   y) with
   | (true, false) => false
@@ -24,9 +25,9 @@ Definition implb(x:bool) (y:bool): bool := match (x,
 Parameter set : forall (a:Type), Type.
 
 Parameter mem: forall (a:Type), a -> (set a) -> Prop.
-
 Implicit Arguments mem.
 
+(* Why3 assumption *)
 Definition infix_eqeq (a:Type)(s1:(set a)) (s2:(set a)): Prop :=
   forall (x:a), (mem x s1) <-> (mem x s2).
 Implicit Arguments infix_eqeq.
@@ -34,6 +35,7 @@ Implicit Arguments infix_eqeq.
 Axiom extensionality : forall (a:Type), forall (s1:(set a)) (s2:(set a)),
   (infix_eqeq s1 s2) -> (s1 = s2).
 
+(* Why3 assumption *)
 Definition subset (a:Type)(s1:(set a)) (s2:(set a)): Prop := forall (x:a),
   (mem x s1) -> (mem x s2).
 Implicit Arguments subset.
@@ -42,25 +44,23 @@ Axiom subset_trans : forall (a:Type), forall (s1:(set a)) (s2:(set a))
   (s3:(set a)), (subset s1 s2) -> ((subset s2 s3) -> (subset s1 s3)).
 
 Parameter empty: forall (a:Type), (set a).
-
 Set Contextual Implicit.
 Implicit Arguments empty.
 Unset Contextual Implicit.
 
+(* Why3 assumption *)
 Definition is_empty (a:Type)(s:(set a)): Prop := forall (x:a), ~ (mem x s).
 Implicit Arguments is_empty.
 
-Axiom empty_def1 : forall (a:Type), (is_empty (empty:(set a))).
+Axiom empty_def1 : forall (a:Type), (is_empty (empty :(set a))).
 
 Parameter add: forall (a:Type), a -> (set a) -> (set a).
-
 Implicit Arguments add.
 
 Axiom add_def1 : forall (a:Type), forall (x:a) (y:a), forall (s:(set a)),
   (mem x (add y s)) <-> ((x = y) \/ (mem x s)).
 
 Parameter remove: forall (a:Type), a -> (set a) -> (set a).
-
 Implicit Arguments remove.
 
 Axiom remove_def1 : forall (a:Type), forall (x:a) (y:a) (s:(set a)), (mem x
@@ -70,21 +70,18 @@ Axiom subset_remove : forall (a:Type), forall (x:a) (s:(set a)),
   (subset (remove x s) s).
 
 Parameter union: forall (a:Type), (set a) -> (set a) -> (set a).
-
 Implicit Arguments union.
 
 Axiom union_def1 : forall (a:Type), forall (s1:(set a)) (s2:(set a)) (x:a),
   (mem x (union s1 s2)) <-> ((mem x s1) \/ (mem x s2)).
 
 Parameter inter: forall (a:Type), (set a) -> (set a) -> (set a).
-
 Implicit Arguments inter.
 
 Axiom inter_def1 : forall (a:Type), forall (s1:(set a)) (s2:(set a)) (x:a),
   (mem x (inter s1 s2)) <-> ((mem x s1) /\ (mem x s2)).
 
 Parameter diff: forall (a:Type), (set a) -> (set a) -> (set a).
-
 Implicit Arguments diff.
 
 Axiom diff_def1 : forall (a:Type), forall (s1:(set a)) (s2:(set a)) (x:a),
@@ -93,8 +90,20 @@ Axiom diff_def1 : forall (a:Type), forall (s1:(set a)) (s2:(set a)) (x:a),
 Axiom subset_diff : forall (a:Type), forall (s1:(set a)) (s2:(set a)),
   (subset (diff s1 s2) s1).
 
-Parameter cardinal: forall (a:Type), (set a) -> Z.
+Parameter choose: forall (a:Type), (set a) -> a.
+Implicit Arguments choose.
 
+Axiom choose_def : forall (a:Type), forall (s:(set a)), (~ (is_empty s)) ->
+  (mem (choose s) s).
+
+Parameter all: forall (a:Type), (set a).
+Set Contextual Implicit.
+Implicit Arguments all.
+Unset Contextual Implicit.
+
+Axiom all_def : forall (a:Type), forall (x:a), (mem x (all :(set a))).
+
+Parameter cardinal: forall (a:Type), (set a) -> Z.
 Implicit Arguments cardinal.
 
 Axiom cardinal_nonneg : forall (a:Type), forall (s:(set a)),
@@ -116,7 +125,7 @@ Parameter vertex : Type.
 
 Parameter succ: vertex -> (set vertex).
 
-
+(* Why3 assumption *)
 Inductive path : vertex -> vertex -> Z -> Prop :=
   | path_empty : forall (v:vertex), (path v v 0%Z)
   | path_succ : forall (v1:vertex) (v2:vertex) (v3:vertex) (n:Z), (path v1 v2
@@ -134,22 +143,27 @@ Axiom path_closure : forall (s:(set vertex)), (forall (x:vertex), (mem x
   forall (v1:vertex) (v2:vertex) (n:Z), (path v1 v2 n) -> ((mem v1 s) ->
   (mem v2 s)).
 
+(* Why3 assumption *)
 Definition shortest_path(v1:vertex) (v2:vertex) (n:Z): Prop := (path v1 v2
   n) /\ forall (m:Z), (m <  n)%Z -> ~ (path v1 v2 m).
 
+(* Why3 assumption *)
 Inductive ref (a:Type) :=
   | mk_ref : a -> ref a.
 Implicit Arguments mk_ref.
 
-Definition contents (a:Type)(u:(ref a)): a :=
-  match u with
-  | (mk_ref contents1) => contents1
+(* Why3 assumption *)
+Definition contents (a:Type)(v:(ref a)): a :=
+  match v with
+  | (mk_ref x) => x
   end.
 Implicit Arguments contents.
 
-Definition bag (a:Type) := (ref (set a)).
+(* Why3 assumption *)
+Definition t (a:Type) := (ref (set a)).
 
-Definition inv(s:vertex) (t:vertex) (visited:(set vertex)) (current:(set
+(* Why3 assumption *)
+Definition inv(s:vertex) (t1:vertex) (visited:(set vertex)) (current:(set
   vertex)) (next:(set vertex)) (d:Z): Prop := (subset current visited) /\
   ((forall (x:vertex), (mem x current) -> (shortest_path s x d)) /\
   ((subset next visited) /\ ((forall (x:vertex), (mem x next) ->
@@ -157,29 +171,29 @@ Definition inv(s:vertex) (t:vertex) (visited:(set vertex)) (current:(set
   m) -> ((m <= d)%Z -> (mem x visited))) /\ ((forall (x:vertex), (mem x
   visited) -> exists m:Z, (path s x m) /\ (m <= (d + 1%Z)%Z)%Z) /\
   ((forall (x:vertex), (shortest_path s x (d + 1%Z)%Z) -> ((mem x next) \/
-  ~ (mem x visited))) /\ ((mem t visited) -> ((mem t current) \/ (mem t
+  ~ (mem x visited))) /\ ((mem t1 visited) -> ((mem t1 current) \/ (mem t1
   next))))))))).
 
+(* Why3 assumption *)
 Definition closure(visited:(set vertex)) (current:(set vertex)) (next:(set
   vertex)) (x:vertex): Prop := (mem x visited) -> ((~ (mem x current)) ->
   ((~ (mem x next)) -> forall (y:vertex), (mem y (succ x)) -> (mem y
   visited))).
 
-(* YOU MAY EDIT THE CONTEXT BELOW *)
 
-(* DO NOT EDIT BELOW *)
 
-Theorem WP_parameter_bfs : forall (s:vertex), forall (t:vertex),
+(* Why3 goal *)
+Theorem WP_parameter_bfs : forall (s:vertex), forall (t1:vertex),
   forall (d:Z), forall (next:(set vertex)), forall (current:(set vertex)),
-  forall (visited:(set vertex)), ((inv s t visited current next d) /\
+  forall (visited:(set vertex)), ((inv s t1 visited current next d) /\
   (((is_empty current) -> (is_empty next)) /\ ((forall (x:vertex),
   (closure visited current next x)) /\ (0%Z <= d)%Z))) ->
   forall (result:bool), ((result = true) <-> (is_empty current)) ->
-  ((result = true) -> ((~ (mem t visited)) -> forall (d1:Z), ~ (path s t
+  ((result = true) -> ((~ (mem t1 visited)) -> forall (d1:Z), ~ (path s t1
   d1))).
 (* YOU MAY EDIT THE PROOF BELOW *)
 intuition.
-assert (mem t visited).
+assert (mem t1 visited).
 apply path_closure with s d1; auto.
 unfold closure in H1.
 intros x hx.
@@ -192,6 +206,5 @@ apply path_empty.
 assumption.
 exact (H5 H8).
 Qed.
-(* DO NOT EDIT BELOW *)
 
 
